examples/map/MapA.v
@@ -8,7 +8,6 @@ Require Import Skeleton.
 Require Import PCM.
 Require Import HoareDef STB IPM.
 Require Import MapHeader.
-
 Require Import sProp sWorld World SRF.
 
 Set Implicit Arguments.
@@ -73,7 +72,7 @@ Section A.
 
   Definition SMapSem: SModSem.t := {|
     SModSem.fnsems := MapSbtb;
-    SModSem.initial_cond := OwnM (Excl.unit, Auth.excl ((fun _ => Excl.just 0%Z): @URA.car (Z ==> (Excl.t Z))%ra) ((fun _ => Excl.just 0%Z): @URA.car (Z ==> (Excl.t Z))%ra));
+    SModSem.initial_cond := Map_initial_cond;
     (* SModSem.initial_mr := GRA.embed (Excl.unit, Auth.excl ((fun _ => Excl.just 0%Z): @URA.car (Z ==> (Excl.t Z))%ra) ((fun _ => Excl.just 0%Z): @URA.car (Z ==> (Excl.t Z))%ra)); *)
     SModSem.initial_st := Ret (fun (_: Z) => 0%Z)↑;
   |}
